PropositionalLogic/KripkeSemantics.v
@@ -1,0 +1,182 @@
+Require Import Logic.LogicBase.
+Require Import Logic.SyntacticReduction.
+Require Import Logic.PropositionalLogic.Syntax.
+Require Import Coq.Logic.Classical_Prop.
+Require Import Coq.Classes.RelationClasses.
+
+Module KripkeSemantics.
+
+Import PropositionalLanguage.
+
+Record frame: Type := {
+  frame_type: Type;
+  frame_order: relation frame_type; (* <= *)
+  frame_preorder: PreOrder frame_order;
+  frame_partialorder: PartialOrder eq frame_order
+}.
+
+Infix "<=" := (frame_order _): KripkeSemantics.
+
+Local Open Scope KripkeSemantics.
+
+Definition sem (f: frame) := sig (fun s: Ensemble (frame_type f) => forall x y, x <= y -> s y -> s x).
+
+Program Definition sem_and {f: frame} (X: sem f) (Y: sem f): sem f :=
+  fun x: frame_type f => X x /\ Y x.
+Next Obligation.
+  split.
+  + eapply (proj2_sig X); eauto.
+  + eapply (proj2_sig Y); eauto.
+Qed.
+
+Program Definition sem_or {f: frame} (X: sem f) (Y: sem f): sem f :=
+  fun x: frame_type f => X x \/ Y x.
+Next Obligation.
+  destruct H0; [left | right].
+  + eapply (proj2_sig X); eauto.
+  + eapply (proj2_sig Y); eauto.
+Qed.
+
+Program Definition sem_imp {f: frame} (X: sem f) (Y: sem f): sem f :=
+  fun x: frame_type f =>
+    forall y: frame_type f, y <= x -> X y -> Y y.
+Next Obligation.
+  revert H2; apply H0.
+  pose proof @PreOrder_Transitive _ _ (frame_preorder f).
+  transitivity x; auto.
+Qed.
+
+Program Definition sem_true {f: frame}: sem f :=
+  fun x: frame_type f => True.
+
+Program Definition sem_false {f: frame}: sem f :=
+  fun x: frame_type f => False.
+
+Definition sem_neg {f: frame} (X: sem f): sem f :=
+  sem_imp X sem_false.
+
+Definition sem_iff {f: frame} (X: sem f) (Y: sem f): sem f :=
+  sem_and (sem_imp X Y) (sem_imp Y X).
+
+Definition denotation {Var: Type} (f: frame) (eval: Var -> sem f): expr Var -> sem f :=
+  fix denotation (x: expr Var): sem f:=
+  match x with
+  | andp y z => sem_and (denotation y) (denotation z)
+  | orp y z => sem_or (denotation y) (denotation z)
+  | impp y z => sem_imp (denotation y) (denotation z)
+  | iffp y z => sem_iff (denotation y) (denotation z)
+  | negp y => sem_neg (denotation y)
+  | truep => sem_true
+  | falsep => sem_false
+  | varp p => eval p
+  end.
+
+Record model {Var: Type} : Type := {
+  model_frame: frame;
+  model_var: Var -> sem model_frame;
+  elm: frame_type model_frame
+}.
+
+Implicit Arguments model.
+
+Instance SM (Var: Type): Semantics (PropositionalLanguage.L Var) :=
+  Build_Semantics (PropositionalLanguage.L Var) (model Var) (fun m x => proj1_sig (denotation (model_frame m) (model_var m) x) (elm m)).
+
+Local Open Scope logic_base.
+Local Open Scope PropositionalLogic.
+
+Lemma ImpAndOrAsPrime_consistent {Var: Type}:
+  forall x y: expr Var,
+    @ImpAndOrAsPrime.atomic_reduce (L Var) (nL Var) (pL Var) x y ->
+    forall f eval v, proj1_sig (denotation f eval x) v <-> proj1_sig (denotation f eval y) v.
+Proof.
+  intros; split; intros; destruct H; auto.
+Qed.
+
+Lemma ReduceIff_consistent {Var: Type}:
+  forall x y: expr Var,
+    @ReduceIff.atomic_reduce (L Var) (nL Var) (pL Var) x y ->
+    forall f eval v, proj1_sig (denotation f eval x) v <-> proj1_sig (denotation f eval y) v.
+Proof.
+  intros; split; intros; destruct H; auto.
+Qed.
+
+Lemma ReduceTrue_consistent {Var: Type}:
+  forall x y: expr Var,
+    @ReduceTrue.atomic_reduce (L Var) (nL Var) (pL Var) x y ->
+    forall f eval v, proj1_sig (denotation f eval x) v <-> proj1_sig (denotation f eval y) v.
+Proof.
+  intros; split; intros; destruct H.
+  + hnf; intros; auto.
+  + hnf; auto.
+Qed.
+
+Lemma disjunction_reduce_consistent {Var: Type}:
+  forall reduce1 reduce2: relation (expr Var),
+    (forall x y, reduce1 x y -> forall f eval v, proj1_sig (denotation f eval x) v <-> proj1_sig (denotation f eval y) v) ->
+    (forall x y, reduce2 x y -> forall f eval v, proj1_sig (denotation f eval x) v <-> proj1_sig (denotation f eval y) v) ->
+    forall x y, relation_disjunction reduce1 reduce2 x y ->
+    forall f eval v, proj1_sig (denotation f eval x) v <-> proj1_sig (denotation f eval y) v.
+Proof.
+  intros.
+  destruct H1.
+  + apply H; auto.
+  + apply H0; auto.
+Qed.
+
+Lemma propag_reduce_consistent {Var: Type}:
+  forall reduce: relation (expr Var),
+    (forall x y, reduce x y -> forall f eval v, proj1_sig (denotation f eval x) v <-> proj1_sig (denotation f eval y) v) ->
+    (forall x y, @propag_reduce (L Var) reduce x y -> forall f eval v, proj1_sig (denotation f eval x) v <-> proj1_sig (denotation f eval y) v).
+Proof.
+  intros.
+  destruct H0.
+  revert v; induction p as [| [| | | | | | | |]]; intros.
+  + simpl; apply H; auto.
+  + specialize (IHp v).
+    simpl in *.
+    tauto.
+  + specialize (IHp v).
+    simpl in *.
+    tauto.
+  + specialize (IHp v).
+    simpl in *.
+    tauto.
+  + specialize (IHp v).
+    simpl in *.
+    tauto.
+  + simpl in *.
+    split; intros HH u Hu; specialize (HH u Hu); specialize (IHp u); tauto.
+  + simpl in *.
+    split; intros HH u Hu; specialize (HH u Hu); specialize (IHp u); tauto.
+  + simpl in *.
+    apply Morphisms_Prop.and_iff_morphism.
+    - simpl in *.
+      split; intros HH u Hu; specialize (HH u Hu); specialize (IHp u); tauto.
+    - simpl in *.
+      split; intros HH u Hu; specialize (HH u Hu); specialize (IHp u); tauto.
+  + simpl in *.
+    apply Morphisms_Prop.and_iff_morphism.
+    - simpl in *.
+      split; intros HH u Hu; specialize (HH u Hu); specialize (IHp u); tauto.
+    - simpl in *.
+      split; intros HH u Hu; specialize (HH u Hu); specialize (IHp u); tauto.
+  + simpl in *.
+    split; intros HH u Hu; specialize (HH u Hu); specialize (IHp u); tauto.
+Qed.
+
+Lemma intuitionistic_consistent {Var: Type}: reduction_consistent_semantics IntuitionisticReduction (SM Var).
+Proof.
+  apply reduction_consistent_semantics_spec.
+  simpl.
+  intros.
+  destruct m as [f eval v]; simpl.
+  revert x y H f eval v; apply propag_reduce_consistent.
+  repeat apply disjunction_reduce_consistent.
+  + apply ImpAndOrAsPrime_consistent.
+  + apply ReduceIff_consistent.
+  + apply ReduceTrue_consistent.
+Qed.
+
+End KripkeSemantics.
+
