Makefile
@@ -6,6 +6,8 @@ COQC = coqc
 
 all: Wf.vo base.vo IPC.vo trivial.vo Kripke.vo enumerate.vo LogicBase.vo SyntacticReduction.v \
      HenkinCompleteness.v PropositionalLogic/MinimunPropositionalLogic.vo \
+     PropositionalLogic/IntuitionisticPropositionalLogic.vo \
+     PropositionalLogic/KripkeSemantics.vo \
      PropositionalLogic/Syntax.vo PropositionalLogic/ClassicalPropositionalLogic.vo \
      PropositionalLogic/TrivialSemantics.vo PropositionalLogic/Sound_Classical_Trivial.vo \
      PropositionalLogic/Complete_Classical_Trivial.vo lib/Coqlib.vo
